Progress is slow :(

Bytestring/Decode.lean
@@ -4,10 +4,10 @@ section decode
 
 inductive FirstByte where
   | invalid : FirstByte
-  | done : (b : UInt8) → b < 0x80 → FirstByte
-  | oneMore : (b : UInt8) → b < 0x20 → FirstByte
-  | twoMore : (b : UInt8) → b < 0x10 → FirstByte
-  | threeMore : (b : UInt8) → b < 0x08 → FirstByte
+  | done : FirstByte
+  | oneMore : FirstByte
+  | twoMore : FirstByte
+  | threeMore : FirstByte
 
 inductive LaterByte where
   | invalid : LaterByte
@@ -75,59 +75,68 @@ theorem UInt8.and_lt_add_one {b c : UInt8} (h : c ≠ -1) : b &&& c < c + 1 :=
 
 @[inline]
 def parseFirstByte (b : UInt8) : FirstByte :=
-  if h : b < 128 then
-    .done b h
+  if b < 128 then
+    .done
   else if b &&& 0xe0 == 0xc0 then
-    .oneMore (b &&& 0x1f) (UInt8.and_lt_add_one (by decide))
+    .oneMore
   else if b &&& 0xf0 == 0xe0 then
-    .twoMore (b &&& 0x0f) (UInt8.and_lt_add_one (by decide))
+    .twoMore
   else if b &&& 0xf8 == 0xf0 then
-    .threeMore (b &&& 0x07) (UInt8.and_lt_add_one (by decide))
+    .threeMore
   else .invalid
 
-theorem parseFirstByte_eq_done (b : UInt8) (hb : b ≤ 127) : parseFirstByte b = .done b (by grind only) := by
+theorem parseFirstByte_eq_done (b : UInt8) (hb : b ≤ 127) : parseFirstByte b = .done := by
   grind [parseFirstByte]
 
 theorem parseFirstByte_eq_oneMore (b : UInt8) (hb₁ : 128 ≤ b) (hb₂ : b &&& 0xe0 = 0xc0) :
-    parseFirstByte b = .oneMore (b &&& 0x1f) (UInt8.and_lt_add_one (by decide)) := by
+    parseFirstByte b = .oneMore := by
   grind [parseFirstByte]
 
 @[inline]
-def parseLaterByte (b : UInt8) : LaterByte :=
-  if b &&& 0xc0 == 0x80 then
-    .valid (b &&& 0x3f) (UInt8.and_lt_add_one (by decide))
-  else .invalid
+def isInvalidContinuationByte (b : UInt8) : Bool :=
+  b &&& 0xc0 != 0x80
 
-theorem parseLaterByte_eq_valid (b : UInt8) (hb : b &&& 0xc0 = 0x80) :
-    parseLaterByte b = .valid (b &&& 0x3f) (UInt8.and_lt_add_one (by decide)) := by
-  grind [parseLaterByte]
+theorem isInvalidContinutationByte_eq_false_iff {b : UInt8} :
+    isInvalidContinuationByte b = false ↔ b &&& 0xc0 = 0x80 := by
+  simp [isInvalidContinuationByte]
+
+-- @[inline]
+-- def parseLaterByte (b : UInt8) : LaterByte :=
+--   if b &&& 0xc0 == 0x80 then
+--     .valid (b &&& 0x3f) (UInt8.and_lt_add_one (by decide))
+--   else .invalid
+
+-- theorem parseLaterByte_eq_valid (b : UInt8) (hb : b &&& 0xc0 = 0x80) :
+--     parseLaterByte b = .valid (b &&& 0x3f) (UInt8.and_lt_add_one (by decide)) := by
+--   grind [parseLaterByte]
 
 @[inline]
 def utf8DecodeChar? (bytes : ByteArray) (i : Nat) : Option Char :=
   if h₀ : i < bytes.size then
-    match parseFirstByte bytes[i] with
+    match h : parseFirstByte bytes[i] with
     | .invalid => none -- invalid first byte
-    | .done b₀ hb₀ => some ⟨b₀.toUInt32, ?done⟩
-    | .oneMore b₀ hb₀ =>
-      if h₁ : i + 1 < bytes.size then
-        match parseLaterByte bytes[i + 1] with
-        | .invalid => none -- invalid second byte
-        | .valid b₁ hb₁ =>
+    | .done => some ⟨bytes[i].toUInt32, ?done⟩
+    | .oneMore =>
+      let b₀ : UInt8 := bytes[i] &&& 0x1f
+      if h₁ : i +  1 < bytes.size then
+        if isInvalidContinuationByte bytes[i + 1] then
+          none
+        else
+          let b₁ := bytes[i + 1] &&& 0x3f
           let r := (b₀.toUInt32 <<< 6) ||| b₁.toUInt32
           if r < 0x80 then
             none -- overlong encoding
           else
             some ⟨r, ?onemore⟩
       else none
-    | .twoMore b₀ hb₀ =>
+    | .twoMore =>
+      let b₀ : UInt8 := bytes[i] &&& 0x0f
       if h₁ : i + 2 < bytes.size then
-        let c₁ := bytes[i + 1]
-        let c₂ := bytes[i + 2]
-        match parseLaterByte bytes[i + 1], parseLaterByte bytes[i + 2] with
-        | .invalid, .invalid => none -- invalid second/third byte
-        | .valid _ _, .invalid => none -- invalid third byte
-        | .invalid, .valid _ _ => none -- invalid second byte
-        | .valid b₁ hb₁, .valid b₂ hb₂ =>
+        if isInvalidContinuationByte bytes[i + 1] || isInvalidContinuationByte bytes[i + 2] then
+          none
+        else
+          let b₁ := bytes[i + 1] &&& 0x3f
+          let b₂ := bytes[i + 2] &&& 0x3f
           let r := (b₀.toUInt32 <<< 12) ||| (b₁.toUInt32 <<< 6) ||| b₂.toUInt32
           if r < 0x800 then
             none -- overlong encoding
@@ -136,20 +145,15 @@ def utf8DecodeChar? (bytes : ByteArray) (i : Nat) : Option Char :=
           else
             some ⟨r, ?twomore⟩
       else none
-    | .threeMore b₀ hb₀ =>
+    | .threeMore =>
+      let b₀ : UInt8 := bytes[i] &&& 0x07
       if h₁ : i + 3 < bytes.size then
-        let c₁ := bytes[i + 1]
-        let c₂ := bytes[i + 2]
-        let c₃ := bytes[i + 3]
-        match parseLaterByte bytes[i + 1], parseLaterByte bytes[i + 2], parseLaterByte bytes[i + 3] with
-        | .invalid, .invalid, .invalid => none -- invalid second/third/fourth byte
-        | .valid _ _, .invalid, .invalid => none -- invalid third/fouth byte
-        | .invalid, .valid _ _, .invalid => none -- invalid second/fourth byte
-        | .valid _ _, .valid _ _, .invalid => none -- invalid fourth byte
-        | .invalid, .invalid, .valid _ _ => none -- invalid second/third byte
-        | .valid _ _, .invalid, .valid _ _ => none -- invalid third byte
-        | .invalid, .valid _ _, .valid _ _ => none -- invalid second byte
-        | .valid b₁ hb₁, .valid b₂ hb₂, .valid b₃ hb₃ =>
+        if isInvalidContinuationByte bytes[i + 1] || isInvalidContinuationByte bytes[i + 2] || isInvalidContinuationByte bytes[i + 3] then
+          none
+        else
+          let b₁ := bytes[i + 1] &&& 0x3f
+          let b₂ := bytes[i + 2] &&& 0x3f
+          let b₃ := bytes[i + 3] &&& 0x3f
           let r := (b₀.toUInt32 <<< 18) ||| (b₁.toUInt32 <<< 12) ||| (b₂.toUInt32 <<< 6) ||| b₃.toUInt32
           if h₁ : r < 0x10000 then
             none -- overlong encoding
@@ -160,8 +164,10 @@ def utf8DecodeChar? (bytes : ByteArray) (i : Nat) : Option Char :=
       else none
   else none
 where finally
-  case done => grind [UInt8.lt_iff_toNat_lt, UInt8.toNat_toUInt32]
+  case done => grind [parseFirstByte, UInt8.lt_iff_toNat_lt, UInt8.toNat_toUInt32]
   case onemore =>
+    have hb₀ : b₀ < 0x20 := UInt8.and_lt_add_one (by decide)
+    have hb₁ : b₁ < 0x40 := UInt8.and_lt_add_one (by decide)
     refine Or.inl ?_
     subst r
     simp only [UInt8.lt_iff_toNat_lt, UInt8.reduceToNat] at hb₀ hb₁
@@ -170,6 +176,9 @@ where finally
     rw [Nat.shiftLeft_eq, Nat.mod_eq_of_lt (by omega), Nat.mul_comm, ← Nat.two_pow_add_eq_or_of_lt hb₁]
     omega
   case twomore =>
+    have hb₀ : b₀ < 0x10 := UInt8.and_lt_add_one (by decide)
+    have hb₁ : b₁ < 0x40 := UInt8.and_lt_add_one (by decide)
+    have hb₂ : b₂ < 0x40 := UInt8.and_lt_add_one (by decide)
     simp only [UInt8.lt_iff_toNat_lt, UInt8.reduceToNat] at hb₀ hb₁ hb₂
     simp only [Decidable.not_and_iff_not_or_not, UInt32.not_le] at hr
     rcases hr with (hr|hr)
@@ -183,6 +192,10 @@ where finally
           ← Nat.two_pow_add_eq_or_of_lt (by omega)]
       omega
   case threemore =>
+    have hb₀ : b₀ < 0x08 := UInt8.and_lt_add_one (by decide)
+    have hb₁ : b₁ < 0x40 := UInt8.and_lt_add_one (by decide)
+    have hb₂ : b₂ < 0x40 := UInt8.and_lt_add_one (by decide)
+    have hb₃ : b₃ < 0x40 := UInt8.and_lt_add_one (by decide)
     simp only [UInt8.lt_iff_toNat_lt, UInt8.reduceToNat] at hb₀ hb₁ hb₂ hb₃
     simp only [UInt32.not_lt, UInt32.le_iff_toNat_le, UInt32.reduceToNat] at h₁ h₂
     exact Or.inr ⟨by omega, by omega⟩
@@ -195,44 +208,115 @@ theorem utf8DecodeChar?_utf8EncodeChar_append {b : ByteArray} {c : Char} :
   fun_cases String.utf8EncodeChar c with
   | case1 v h =>
     rw [utf8DecodeChar?, dif_pos (by simp; grind [Char.utf8Size_pos])]
-    rw [parseFirstByte_eq_done]
+    have : parseFirstByte ([v.toUInt8].toByteArray ++ b)[0] = .done := by
+      rw [parseFirstByte_eq_done]
+      simp [UInt8.le_iff_toNat_le, UInt32.le_iff_toNat_le] at h ⊢
+      grind
+    split <;> rename_i h' <;> try (simp_all; done)
     · simp only [Option.some.injEq]
       ext
       simp
       grind
-    · simp [UInt8.le_iff_toNat_le, UInt32.le_iff_toNat_le] at h ⊢
-      grind
   | case2 v h₁ h₂ =>
     rw [utf8DecodeChar?, dif_pos (by simp; grind [Char.utf8Size_pos])]
-    rw [parseFirstByte_eq_oneMore]
-    · simp only
-      rw [dif_pos (by simp; grind)]
-      simp only [Nat.zero_add, List.size_toByteArray, List.length_cons, List.length_nil,
-        Nat.reduceAdd, Nat.lt_add_one, ByteArray.getElem_append_left, List.getElem_toByteArray,
-        List.getElem_cons_succ, List.getElem_cons_zero, Nat.zero_lt_succ, UInt8.toUInt32_and,
-        UInt8.toUInt32_or, UInt32.toUInt32_toUInt8, Nat.reduceLT, UInt8.toUInt32_ofNat]
-      rw [parseLaterByte_eq_valid]
-      · simp only [UInt8.toUInt32_and, UInt8.toUInt32_or, UInt32.toUInt32_toUInt8, Nat.reduceLT,
-          UInt8.toUInt32_ofNat, Option.ite_none_left_eq_some, UInt32.not_lt, Option.some.injEq]
-        refine ⟨?_, ?_⟩
-        · sorry
-        · ext
-          simp
-          sorry
-      · sorry
-    · simp
-      sorry
-    · simp
-      sorry
+    sorry
+    -- rw [parseFirstByte_eq_oneMore]
+    -- · simp only
+    --   rw [dif_pos (by simp; grind)]
+    --   simp only [Nat.zero_add, List.size_toByteArray, List.length_cons, List.length_nil,
+    --     Nat.reduceAdd, Nat.lt_add_one, ByteArray.getElem_append_left, List.getElem_toByteArray,
+    --     List.getElem_cons_succ, List.getElem_cons_zero, Nat.zero_lt_succ, UInt8.toUInt32_and,
+    --     UInt8.toUInt32_or, UInt32.toUInt32_toUInt8, Nat.reduceLT, UInt8.toUInt32_ofNat]
+    --   rw [parseLaterByte_eq_valid]
+    --   · simp only [UInt8.toUInt32_and, UInt8.toUInt32_or, UInt32.toUInt32_toUInt8, Nat.reduceLT,
+    --       UInt8.toUInt32_ofNat, Option.ite_none_left_eq_some, UInt32.not_lt, Option.some.injEq]
+    --     refine ⟨?_, ?_⟩
+    --     · sorry
+    --     · ext
+    --       simp
+    --       sorry
+    --   · sorry
+    -- · simp
+    --   sorry
+    -- · simp
+    --   sorry
   | case3 => sorry
   | case4 => sorry
 
+theorem String.utf8EncodeChar_eq_singleton {c : Char} (hc : c.val < 128) :
+    String.utf8EncodeChar c = [c.val.toUInt8] := by
+  grind [utf8EncodeChar]
+
+theorem String.utf8EncodeChar_eq_cons_cons {c : Char} (hc₀ : 128 ≤ c.val) (hc₁ : c.val ≤ 0x7ff) :
+    String.utf8EncodeChar c = [(c.val >>>  6).toUInt8 &&& 0x1f ||| 0xc0, c.val.toUInt8 &&& 0x3f ||| 0x80] := by
+  grind [utf8EncodeChar]
+
+theorem String.utf8EncodeChar_eq_cons_cons_cons {c : Char} (hc₀ : 0x7ff < c.val) (hc₁ : c.val ≤ 0xffff) :
+    String.utf8EncodeChar c =
+    [(c.val >>> 12).toUInt8 &&& 0x0f ||| 0xe0,
+     (c.val >>>  6).toUInt8 &&& 0x3f ||| 0x80,
+              c.val.toUInt8 &&& 0x3f ||| 0x80] := by
+  grind [utf8EncodeChar]
+
+theorem String.utf8EncodeChar_eq_cons_cons_cons_cons {c : Char} (hc : 0xffff < c.val) :
+    String.utf8EncodeChar c =
+    [(c.val >>> 18).toUInt8 &&& 0x07 ||| 0xf0,
+     (c.val >>> 12).toUInt8 &&& 0x3f ||| 0x80,
+     (c.val >>>  6).toUInt8 &&& 0x3f ||| 0x80,
+              c.val.toUInt8 &&& 0x3f ||| 0x80] := by
+  grind [utf8EncodeChar]
+
 theorem eq_of_utf8DecodeChar?_eq_some {b : ByteArray} {c : Char} (h : utf8DecodeChar? b 0 = some c) :
     b = (String.utf8EncodeChar c).toByteArray ++ b.extract c.utf8Size b.size := by
-  ext
-  simp
-  sorry
-  sorry
+  conv => lhs; rw [← ByteArray.extract_zero_size (b := b), ByteArray.extract_eq_extract_append_extract (min c.utf8Size b.size) (by simp) (Nat.min_le_right ..)]
+  congr 1
+  · revert h
+    fun_cases utf8DecodeChar? b 0
+    all_goals try (simp; done)
+    all_goals (simp only [Option.some.injEq]); rintro rfl
+    · rename_i hb hp
+      rw [← String.length_utf8EncodeChar, String.utf8EncodeChar_eq_singleton]
+      · simp only [UInt8.toUInt8_toUInt32, List.length_cons, List.length_nil, Nat.zero_add,
+        (by omega : min 1 b.size = 1)]
+        rw [ByteArray.extract_add_one (by omega)]
+      · simp [UInt32.lt_iff_toNat_lt]
+        grind [parseFirstByte, UInt8.lt_iff_toNat_lt]
+    · rename_i _ hp b₀ hb hb₁ b₁ r hr
+      subst b₀ b₁ r
+      rw [← String.length_utf8EncodeChar, String.utf8EncodeChar_eq_cons_cons]
+      · simp [(by omega : min 2 b.size = 2)]
+        rw [ByteArray.extract_add_two (by omega)]
+        congr
+        · sorry
+        · sorry
+      · grind
+      · simp [UInt32.le_iff_toNat_le]
+        · sorry
+    · rename_i _ hp b₀ hb hb₁₂ b₁ b₂ r hr₁ hr₂
+      subst b₀ b₁ b₂ r
+      rw [← String.length_utf8EncodeChar, String.utf8EncodeChar_eq_cons_cons_cons]
+      · simp [(by omega : min 3 b.size = 3)]
+        rw [ByteArray.extract_add_three (by omega)]
+        congr
+        · sorry
+        · sorry
+        · sorry
+      · grind
+      · sorry
+    · rename_i _ hp b₀ hb hb₁₂₃ b₁ b₂ b₃ r hr₁ hr₂
+      subst b₀ b₁ b₂ b₃ r
+      rw [← String.length_utf8EncodeChar, String.utf8EncodeChar_eq_cons_cons_cons_cons]
+      · simp [(by omega : min 4 b.size = 4)]
+        rw [ByteArray.extract_add_four (by omega)]
+        simp [isInvalidContinutationByte_eq_false_iff] at hb₁₂₃
+        congr
+        · sorry
+        · sorry
+        · sorry
+        · sorry
+      · grind
+  · simp only [ByteArray.extract_eq_extract_left, Nat.le_refl, Nat.min_eq_left]
+    omega
 
 theorem exists_of_utf8DecodeChar?_eq_some {b : ByteArray} {c : Char} (h : utf8DecodeChar? b 0 = some c) :
     ∃ l, b = (String.utf8EncodeChar c).toByteArray ++ l :=
@@ -241,16 +325,38 @@ theorem exists_of_utf8DecodeChar?_eq_some {b : ByteArray} {c : Char} (h : utf8De
 theorem utf8DecodeChar?_eq_utf8DecodeChar?_drop {b : ByteArray} {i : Nat} :
     utf8DecodeChar? b i = utf8DecodeChar? (b.extract i b.size) 0 := by
   simp [utf8DecodeChar?]
-  have : i < b.size ↔ 0 < b.size - i := by omega
-  have : i + 1 < b.size ↔ 1 < b.size - i := by omega
-  have : i + 2 < b.size ↔ 2 < b.size - i := by omega
-  have : i + 3 < b.size ↔ 3 < b.size - i := by omega
-  have : ∀ h h', b[i]'h = (b.extract i b.size)[0]'h' := by simp [ByteArray.getElem_extract]
-  have : ∀ h h', b[i + 1]'h = (b.extract i b.size)[1]'h' := by simp [ByteArray.getElem_extract]
-  have : ∀ h h', b[i + 2]'h = (b.extract i b.size)[2]'h' := by simp [ByteArray.getElem_extract]
-  have : ∀ h h', b[i + 3]'h = (b.extract i b.size)[3]'h' := by simp [ByteArray.getElem_extract]
-  have : (b.extract i b.size).size = b.size - i := by simp
-  grind
+  have h₁ : i < b.size ↔ 0 < b.size - i := by omega
+  have h₂ : i + 1 < b.size ↔ 1 < b.size - i := by omega
+  have h₃ : i + 2 < b.size ↔ 2 < b.size - i := by omega
+  have h₄ : i + 3 < b.size ↔ 3 < b.size - i := by omega
+  have h₅ : ∀ h, b[i]'h = (b.extract i b.size)[0]'(by simp; omega) := by simp [ByteArray.getElem_extract]
+  have h₆ : ∀ h, b[i + 1]'h = (b.extract i b.size)[1]'(by simp; omega) := by simp [ByteArray.getElem_extract]
+  have h₇ : ∀ h, b[i + 2]'h = (b.extract i b.size)[2]'(by simp; omega) := by simp [ByteArray.getElem_extract]
+  have h₈ : ∀ h, b[i + 3]'h = (b.extract i b.size)[3]'(by simp; omega) := by simp [ByteArray.getElem_extract]
+  have h₉ : (b.extract i b.size).size = b.size - i := by simp
+  simp only [h₁]
+  split
+  · split
+    all_goals (rename_i h h'; simp only [h₅] at h')
+    · split <;> simp_all
+    · split <;> rename_i h''
+      all_goals try (simp [h'] at h''; done)
+      simp [h₅]
+    · symm
+      split <;> rename_i h''
+      all_goals try (simp [h'] at h''; done)
+      simp [h₂, h₅, h₆]
+    · symm
+      split <;> rename_i h''
+      all_goals try (simp [h'] at h''; done)
+      simp [h₃, h₅, h₆, h₇]
+    · symm
+      split <;> rename_i h''
+      all_goals try (simp [h'] at h''; done)
+      simp [h₄, h₅, h₆, h₇, h₈]
+  · rfl
+
+  -- grind
 
 theorem le_size_of_utf8DecodeChar?_eq_some {b : ByteArray} {i : Nat} {c : Char}
     (h : utf8DecodeChar? b i = some c) : i + c.utf8Size ≤ b.size := by
